\documentclass[12pt,a4paper]{article}
\usepackage[mathjax]{lwarp}
\usepackage{amsmath,amssymb,amsfonts}
\usepackage{geometry}
\usepackage{hyperref}
\usepackage{lipsum}
\usepackage{graphicx}

\geometry{margin=2.5cm}

\title{Equation Playground and Log Page}
\author{}
\date{\today}

\begin{document}
\maketitle
\tableofcontents
\clearpage


\begin{figure}[h!]
  \centering
  \includegraphics[width=\textwidth]{./figures/placeholder1.jpg}
  \caption{System overview of the proposed method's  pipeline}
  \label{fig:systemoverview}
\end{figure}

\begin{abstract}
  \lipsum[3]
  \vline
  Hello
\end{abstract}

\section{Basic Algebra}

A simple quadratic equation:
\begin{equation}
  ax^2 + bx + c = 0,
\end{equation}
with solutions
\begin{equation}
  x = \frac{-b \pm \sqrt{b^2 - 4ac}}{2a}.
\end{equation}

Binomial theorem:
\begin{equation}
  (x + y)^n = \sum_{k=0}^{n} \binom{n}{k} x^{n-k} y^k.
\end{equation}

Geometric series:
\begin{equation}
  \sum_{k=0}^{n} r^k = \frac{1 - r^{n+1}}{1 - r}, \qquad r \neq 1.
\end{equation}

\begin{align}
  (a + b)^2 & = a^2 + 2ab + b^2, \\
  (a - b)^2 & = a^2 - 2ab + b^2, \\
  a^2 - b^2 & = (a - b)(a + b).
\end{align}

\section{Calculus}

Definition of the derivative:
\begin{equation}
  f'(x) = \lim_{h \to 0} \frac{f(x + h) - f(x)}{h}.
\end{equation}

Fundamental theorem of calculus:
\begin{equation}
  \int_{a}^{b} f'(x)\,dx = f(b) - f(a).
\end{equation}

Some common derivatives:
\begin{align}
  \frac{d}{dx} x^n    & = n x^{n-1}, \\
  \frac{d}{dx} e^x    & = e^x,       \\
  \frac{d}{dx} \sin x & = \cos x,    \\
  \frac{d}{dx} \cos x & = -\sin x.
\end{align}

Some common integrals:
\begin{align}
  \int x^n\,dx         & = \frac{x^{n+1}}{n+1} + C, \quad n \neq -1, \\
  \int \frac{1}{x}\,dx & = \ln |x| + C,                              \\
  \int e^x\,dx         & = e^x + C,                                  \\
  \int \sin x\,dx      & = -\cos x + C.
\end{align}

A multivariable integral:
\begin{equation}
  \iint_{D} (x^2 + y^2)\,dA
\end{equation}
over some domain $D \subset \mathbb{R}^2$.

\section{Linear Algebra}

Matrix equation:
\begin{equation}
  A \mathbf{x} = \mathbf{b},
\end{equation}
where
\begin{equation}
  A =
  \begin{bmatrix}
    a_{11} & a_{12} & \cdots & a_{1n} \\
    a_{21} & a_{22} & \cdots & a_{2n} \\
    \vdots & \vdots & \ddots & \vdots \\
    a_{m1} & a_{m2} & \cdots & a_{mn}
  \end{bmatrix},
  \quad
  \mathbf{x} =
  \begin{bmatrix}
    x_1 \\ x_2 \\ \vdots \\ x_n
  \end{bmatrix},
  \quad
  \mathbf{b} =
  \begin{bmatrix}
    b_1 \\ b_2 \\ \vdots \\ b_m
  \end{bmatrix}.
\end{equation}

Determinant of a $2 \times 2$ matrix:
\begin{equation}
  \det
  \begin{bmatrix}
    a & b \\
    c & d
  \end{bmatrix}
  = ad - bc.
\end{equation}

Eigenvalue equation:
\begin{equation}
  A \mathbf{v} = \lambda \mathbf{v}.
\end{equation}

\section{Probability and Statistics}

Probability of event $A$:
\begin{equation}
  P(A) = \frac{\text{number of favorable outcomes}}{\text{total number of outcomes}}.
\end{equation}

Linearity of expectation:
\begin{equation}
  \mathbb{E}\left[\sum_{i=1}^{n} X_i\right]
  = \sum_{i=1}^{n} \mathbb{E}[X_i].
\end{equation}

Variance:
\begin{equation}
  \operatorname{Var}(X) = \mathbb{E}[X^2] - \big(\mathbb{E}[X]\big)^2.
\end{equation}

Normal distribution pdf:
\begin{equation}
  f(x) = \frac{1}{\sqrt{2\pi \sigma^2}}
  \exp\left( -\frac{(x - \mu)^2}{2\sigma^2} \right).
\end{equation}

Bayes' theorem:
\begin{equation}
  P(A \mid B) = \frac{P(B \mid A) P(A)}{P(B)}.
\end{equation}

\clearpage
\section{Logarithms (Log Page)}

Basic definition:
\begin{equation}
  \log_a b = c \quad \Longleftrightarrow \quad a^c = b,
\end{equation}
for $a > 0$, $a \neq 1$, and $b > 0$.

Change of base:
\begin{equation}
  \log_a b = \frac{\log_c b}{\log_c a}.
\end{equation}

\subsection{Logarithm Identities}

For $a > 0$, $a \neq 1$, and $x,y > 0$:
\begin{align}
  \log_a (xy)                     & = \log_a x + \log_a y, \\
  \log_a \left(\frac{x}{y}\right) & = \log_a x - \log_a y, \\
  \log_a (x^k)                    & = k \log_a x,          \\
  \log_a a                        & = 1,                   \\
  \log_a 1                        & = 0.
\end{align}

Natural logarithm:
\begin{equation}
  \ln x = \log_e x.
\end{equation}

Derivative of the natural logarithm:
\begin{equation}
  \frac{d}{dx} \ln x = \frac{1}{x}.
\end{equation}

Derivative of a general logarithm:
\begin{equation}
  \frac{d}{dx} \log_a x = \frac{1}{x \ln a}.
\end{equation}

An integral involving logarithms:
\begin{equation}
  \int \ln x\,dx = x \ln x - x + C.
\end{equation}

\subsection{Logarithmic Equations}

Solve
\begin{equation}
  \log_2 (x - 1) + \log_2 (x + 3) = 4.
\end{equation}

Using the product rule:
\begin{equation}
  \log_2 \big((x - 1)(x + 3)\big) = 4
  \quad \Longrightarrow \quad
  (x - 1)(x + 3) = 2^4 = 16.
\end{equation}

Thus
\begin{equation}
  x^2 + 2x - 3 = 16
  \quad \Longrightarrow \quad
  x^2 + 2x - 19 = 0.
\end{equation}

\subsection{Logarithmic Series}

For $|x| < 1$:
\begin{equation}
  \ln(1 + x) = \sum_{n=1}^{\infty} (-1)^{n+1} \frac{x^n}{n}.
\end{equation}

For $x > -1$, $x \neq 0$:
\begin{equation}
  \ln x = 2 \sum_{n=0}^{\infty}
  \frac{1}{2n+1}
  \left(\frac{x-1}{x+1}\right)^{2n+1}.
\end{equation}

\subsection{A Long Log Page Filler}

Here is some filler text to make this a long page:

\lipsum[1-3]

\end{document}
